***NO_CI*** wip; define sel as (heap -> addr -> Tot int) to make progress; use pointwise in examples to rewrite terms

examples/seplogic/FStar.SepLogic.Heap.fst
@@ -5,19 +5,22 @@ include FStar.Heap
 type addr = ref int
 
 abstract let restrict (h:heap) (r:addr) :heap
-  = admit()
+  = admit ()
 
 abstract let minus (h:heap) (r:addr) :heap
-  = admit()
+  = admit ()
 
 abstract let disjoint_from (h1:heap) (h2:heap) :Type0
-  = admit()
+  = admit ()
 
 abstract let join (h1:heap) (h2:heap) :heap
-  = admit()
+  = admit ()
 
 abstract let points_to (r:addr) (x:int) :heap
-  = admit()
+  = admit ()
+
+abstract let sel (h:heap) (r:addr) :Tot int
+  = admit ()
 
 let lemma0 (r:addr) (h:heap)
   :Lemma (requires True)
@@ -29,40 +32,51 @@ let lemma2 (h1:heap) (h2:heap)
   :Lemma (requires True)
          (ensures (h1 `join` h2) == (h2 `join` h1))
 	 [SMTPat (h1 `join` h2)]
-  = admit()
+  = admit ()
 
 let lemma3 (h1:heap) (h2:heap)
   :Lemma (requires True)
          (ensures (h1 `disjoint_from` h2) == (h2 `disjoint_from` h1))
 	 [SMTPat (h1 `disjoint_from` h2)]
-  = admit()
+  = admit ()
 
 let lemma4 (r:addr) (x:int) (h1:heap)
   :Lemma (requires True)
          (ensures sel ((r `points_to` x) `join` h1) r == x)
 	 [SMTPat (sel ((r `points_to` x) `join` h1) r)]
-  = admit()
+  = admit ()
 
 let lemma5 (r:addr) (r1:addr{addr_of r1 <> addr_of r}) (x:int) (h1:heap)
   :Lemma (requires True)
          (ensures sel ((r `points_to` x) `join` h1) r1 == sel h1 r1)
 	 [SMTPat (sel ((r `points_to` x) `join` h1) r1)]
-  = admit()
+  = admit ()
 
 let lemma6 (h:heap)
   :Lemma (requires True)
          (ensures h `join` emp == h)
 	 [SMTPat (h `join` emp)]
-  = admit()
+  = admit ()
 
+let lemma6' (h:heap)
+  :Lemma (requires True)
+         (ensures emp `join` h == h)
+  = admit ()
+  
 let lemma7 (r:addr) (h:heap)
   :Lemma (requires True)
          (ensures (h `restrict` r) == (r `points_to` (sel h r)))
 	 [SMTPat (h `restrict` r)]
-  = admit()
+  = admit ()
 
 let lemma8 (r:addr) (x:int) (y:int)
   :Lemma (requires (points_to r x == points_to r y))
          (ensures  (x == y))
 	 [SMTPat (points_to r x); SMTPat (points_to r y)]
+  = admit ()
+
+let lemma9 (r:addr) (r1:addr{addr_of r1 <> addr_of r})(h:heap)
+  :Lemma (requires True)
+         (ensures sel (minus h r1) r == sel h r)
+         [SMTPat (sel (minus h r1) r)]
   = admit ()
